More work on scoping stuff

src/coq/Syntax/Scope.v
@@ -5,9 +5,12 @@ Import ListNotations.
 
 From Vellvm Require Import
      Numeric.Coqlib
+     Utils.Util
+     Utils.Tactics
      Syntax.LLVMAst
      Syntax.CFG
      Syntax.TypToDtyp.
+
 (* end hide *)
 
 (** * Scoping
@@ -25,16 +28,16 @@ From Vellvm Require Import
 (** * Well-formedness w.r.t. block identifiers
     An [ocfg] should not admit any collisions w.r.t. to its labels.
  *)
-Section OCFG_BID_OPERATIONS.
+Section LABELS_OPERATIONS.
 
-  Context {T : Type}.
+  Context {T : Set}.
 
   (** * inputs
      Collect the list of input labels in an open control flow graph.
      Denoting an [ocfg] starting from a label out of this static list
      always results in the identity.
    *)
-  Definition inputs {t} (ocfg : @ocfg t) :=
+  Definition inputs (ocfg : @ocfg T) :=
     map blk_id ocfg.
 
   (** * outputs
@@ -42,7 +45,7 @@ Section OCFG_BID_OPERATIONS.
      Denoting an [ocfg] starting from a label that belongs to its [inputs]
      will always result in a label in the static [output] list, or in a value.
    *)
-  Definition terminator_outputs {t} (term : LLVMAst.terminator t) : list block_id
+  Definition terminator_outputs (term : terminator T) : list block_id
     := match term with
        | TERM_Ret v => []
        | TERM_Ret_void => []
@@ -54,25 +57,47 @@ Section OCFG_BID_OPERATIONS.
        | TERM_Invoke fnptrval args to_label unwind_label => [to_label; unwind_label]
        end.
 
-  Definition bk_outputs {t} (bk : block t) : list block_id :=
+  Definition bk_outputs (bk : block T) : list block_id :=
     terminator_outputs (snd (blk_term bk)).
 
-  Definition outputs {t} (bks : @ocfg t) : List.list block_id
+  Definition outputs (bks : ocfg T) : list block_id
     := fold_left (fun acc bk => acc ++ bk_outputs bk) bks [].
 
-  (* All labels in a list of blocks are distinct *)
-  Definition wf_ocfg_bid {T} (bks : list (LLVMAst.block T)) :=
+  (** * well-formed
+      All labels in a list of blocks are distinct
+   *)
+  Definition wf_ocfg_bid (bks : ocfg T) : Prop :=
     list_norepet (map blk_id bks).
 
-  (* The  *)
+End LABELS_OPERATIONS.
+
+Section DEF_SITES_OPERATIONS.
+
+  Context {T : Set}.
+
+  Definition def_sites_instr_id (id : instr_id) : list raw_id :=
+    match id with
+    | IId id => [id]
+    | _ => []
+    end.
+
+  Definition def_sites_code (c : code T) : list raw_id :=
+    List.fold_left (fun acc '(id,_) => match id with | IId id => id :: acc | _ => acc end) c [].
+
+End DEF_SITES_OPERATIONS.
+
+Section LABELS_THEORY.
+
+  Context {T : Set}.
+
   Lemma wf_ocfg_bid_nil:
-    forall T, wf_ocfg_bid (T := T) []. 
+    wf_ocfg_bid (T := T) []. 
   Proof.
     intros; apply list_norepet_nil.
   Qed.
 
   Lemma wf_ocfg_bid_cons :
-    forall T (b : LLVMAst.block T) bs,
+    forall (b : block T) bs,
       wf_ocfg_bid (b :: bs) ->
       wf_ocfg_bid bs.
   Proof.
@@ -80,7 +105,7 @@ Section OCFG_BID_OPERATIONS.
   Qed.
 
   Lemma wf_ocfg_bid_cons_not_in :
-    forall T (b : LLVMAst.block T) bs,
+    forall (b : block T) bs,
       wf_ocfg_bid (b :: bs) ->
       not (In (blk_id b) (map blk_id bs)).
   Proof.
@@ -88,7 +113,7 @@ Section OCFG_BID_OPERATIONS.
   Qed.
 
   Lemma wf_ocfg_bid_app_r :
-    forall T (bs1 bs2 : list (LLVMAst.block T)), 
+    forall (bs1 bs2 : ocfg T), 
       wf_ocfg_bid (bs1 ++ bs2) ->
       wf_ocfg_bid bs2.
   Proof.
@@ -100,7 +125,7 @@ Section OCFG_BID_OPERATIONS.
   Qed.
 
   Lemma wf_ocfg_bid_app_l :
-    forall T (bs1 bs2 : list (LLVMAst.block T)), 
+    forall (bs1 bs2 : ocfg T), 
       wf_ocfg_bid (bs1 ++ bs2) ->
       wf_ocfg_bid bs1.
   Proof.
@@ -111,34 +136,205 @@ Section OCFG_BID_OPERATIONS.
     eauto.
   Qed.
 
-  Lemma blk_id_convert_typ : forall env b,
+  Lemma blk_id_convert_typ :
+    forall env b,
       blk_id (convert_typ env b) = blk_id b.
   Proof.
     intros ? []; reflexivity.
   Qed.
 
-  (* Lemma blk_id_map_convert_typ : forall env bs, *)
-  (*     map blk_id (convert_typ env bs) = map blk_id bs. *)
+  (* TODO: Show symmetric case *)
+  Lemma wf_ocfg_bid_app_not_in_l :
+    forall id (bs bs' : ocfg T),
+      In id (inputs bs) ->
+      wf_ocfg_bid (bs' ++ bs) ->
+      not (In id (inputs bs')).
+  Proof.
+    intros. destruct bs.
+    inversion H.
+    inv H.
+    apply wf_ocfg_bid_cons_not_in.
+    unfold wf_ocfg_bid in *.
+    rewrite map_app in H0.
+    rewrite map_cons. rewrite map_cons in H0.
+    rewrite list_cons_app in H0.
+    rewrite app_assoc in H0.
+    apply list_norepet_append_left in H0.
+    rewrite list_cons_app.
+    rewrite list_norepet_app in *.
+    intuition. apply list_disjoint_sym. auto.
+    unfold wf_ocfg_bid in H0.
+    rewrite map_app in H0. rewrite map_cons in H0. rewrite list_cons_app in H0.
+    apply list_norepet_append_commut in H0. rewrite <- app_assoc in H0.
+    apply list_norepet_append_right in H0.
+    rewrite list_norepet_app in H0.
+    destruct H0 as (? & ? & ?).
+    red in H2. intro. eapply H2; eauto.
+  Qed.
+
+  (* TODO: Show symmetric case *)
+  Lemma wf_ocfg_app_not_in_r :
+    forall id (bs bs' : ocfg T),
+      In id (inputs bs) ->
+      wf_ocfg_bid (bs' ++ bs) ->
+      not (In id (inputs bs')).
+  Proof.
+    intros. destruct bs.
+    inversion H.
+    inv H.
+    apply wf_ocfg_bid_cons_not_in.
+    unfold wf_ocfg_bid in *.
+    rewrite map_app in H0.
+    rewrite map_cons. rewrite map_cons in H0.
+    rewrite list_cons_app in H0.
+    rewrite app_assoc in H0.
+    apply list_norepet_append_left in H0.
+    rewrite list_cons_app.
+    rewrite list_norepet_app in *.
+    intuition. apply list_disjoint_sym. auto.
+    unfold wf_ocfg_bid in H0.
+    rewrite map_app in H0. rewrite map_cons in H0. rewrite list_cons_app in H0.
+    apply list_norepet_append_commut in H0. rewrite <- app_assoc in H0.
+    apply list_norepet_append_right in H0.
+    rewrite list_norepet_app in H0.
+    destruct H0 as (? & ? & ?).
+    red in H2. intro. eapply H2; eauto.
+  Qed.
+
+End LABELS_THEORY.
+
+Section FIND_BLOCK.
+
+  Context {T : Set}.
+
+  Lemma find_block_app_r_wf :
+    forall  (x : block_id) (b : block T) (bs1 bs2 : ocfg T),
+      wf_ocfg_bid (bs1 ++ bs2)  ->
+      find_block bs2 x = Some b ->
+      find_block (bs1 ++ bs2) x = Some b.
+  Proof.
+    intros x b; induction bs1 as [| hd bs1 IH]; intros * NOREP FIND.
+    - rewrite app_nil_l; auto.
+    - cbn; break_inner_match_goal.
+      + cbn in *.
+        apply wf_ocfg_bid_cons_not_in in NOREP.
+        exfalso; apply NOREP.
+        rewrite e.
+        apply find_some in FIND as [FIND EQ].
+        clear - FIND EQ.
+        rewrite map_app; eapply in_or_app; right.
+        break_match; [| intuition].
+        rewrite <- e.
+        eapply in_map; auto.
+      + cbn in NOREP; apply wf_ocfg_bid_cons in NOREP.
+        apply IH; eauto.
+  Qed.
+
+  Lemma find_block_app_l_wf :
+    forall (x : block_id) (b : block T) (bs1 bs2 : ocfg T),
+      wf_ocfg_bid (bs1 ++ bs2)  ->
+      find_block bs1 x = Some b ->
+      find_block (bs1 ++ bs2) x = Some b.
+  Proof.
+    intros x b; induction bs1 as [| hd bs1 IH]; intros * NOREP FIND.
+    - inv FIND.
+    - cbn in FIND |- *.
+      break_inner_match; auto.
+      apply IH; eauto.
+      eapply wf_ocfg_bid_cons, NOREP.
+  Qed.
+
+  Lemma find_block_tail_wf :
+    forall (x : block_id) (b b' : block T) (bs : ocfg T),
+      wf_ocfg_bid (b :: bs)  ->
+      find_block bs x = Some b' ->
+      find_block (b :: bs) x = Some b'.
+  Proof.
+    intros.
+    rewrite list_cons_app.
+    apply find_block_app_r_wf; auto.
+  Qed.
+
+  Definition free_in_cfg (cfg : ocfg T ) (id : block_id) : Prop :=
+    not (In id (inputs cfg)).
+
+  Lemma free_in_cfg_cons:
+    forall b (bs : ocfg T) id,
+      free_in_cfg (b::bs) id ->
+      free_in_cfg bs id .
+  Proof.
+    intros * FR abs; apply FR; cbn.
+    destruct (Eqv.eqv_dec_p (blk_id b) id); [rewrite e; auto | right; auto].
+  Qed.
+
+  Lemma find_block_free_id :
+    forall (cfg : ocfg T) id,
+      free_in_cfg cfg id ->
+      find_block cfg id = None.
+  Proof.
+    induction cfg as [| b bs IH]; cbn; intros * FREE; auto.
+    break_inner_match_goal.
+    + exfalso; eapply FREE.
+      cbn; rewrite e; auto.
+    + apply IH.
+      apply free_in_cfg_cons in FREE; auto.
+  Qed.
+
+End FIND_BLOCK.
+
+(* TODO:  *)
+
+  (* Lemma def_sites_modified_instr : forall defs id (i : instr _) g l m, *)
+  (*   interp_cfg_to_L3 defs (denote_instr (id,i)) g l m ⤳ (fun '(_,(l',_)) => forall k, l' @ k <> l @ k -> In k (def_sites_instr_id id)). *)
   (* Proof. *)
-  (*   induction bs as [| b bs IH]; cbn; auto. *)
-  (*   f_equal; auto. *)
-  (* Qed. *)
+  (*   intros. *)
+  (*   destruct i; cbn. *)
+  (*   - rewrite denote_instr_comment; apply eutt_Ret; intros; intuition. *)
+  (*   - destruct id. *)
+  (*     + admit. *)
+  (*     + Transparent denote_instr. *)
+  (*       cbn. *)
+        
+  (*     has_failure *)
+  (*       unfold has_post. *)
+  (*     rewrite denote_instr_op. apply eutt_Ret; intros; intuition. *)
 
-  (* Lemma wf_ocfg_bid_convert_typ : *)
-  (*   forall env (bs : list (LLVMAst.block typ)), *)
-  (*     wf_ocfg_bid bs -> *)
-  (*     wf_ocfg_bid (convert_typ env bs). *)
-  (* Proof. *)
-  (*   induction bs as [| b bs IH]; intros NOREP. *)
-  (*   - cbn; auto. *)
-  (*   - cbn. *)
-  (*     apply list_norepet_cons.  *)
-  (*     + cbn. *)
-  (*       apply wf_ocfg_bid_cons_not_in in NOREP. *)
-  (*       rewrite blk_id_map_convert_typ; auto. *)
-  (*     + eapply IH, wf_ocfg_bid_cons; eauto.  *)
-  (* Qed. *)
+  (*     Lemma def_sites_modified_code : forall defs (c : code _) g l m, *)
+  (*         interp_cfg_to_L3 defs (denote_code c) g l m ⤳ (fun '(_,(l',_)) => forall k, l' @ k <> l @ k -> In k (def_sites_code c)). *)
+  (*     Proof. *)
+  (*       induction c as [| i c IH]; intros. *)
+  (*       - cbn. *)
+  (*         rewrite denote_code_nil, interp_cfg_to_L3_ret. *)
+  (*         apply eutt_Ret. *)
+  (*         intros; auto. *)
+  (*       - cbn. *)
+  (*         rewrite denote_code_cons, interp_cfg_to_L3_bind. *)
+  (*         eapply has_post_bind_strong. *)
+          
+  (*         apply eutt_Ret. *)
+  (*         intros ? abs; auto. *)
 
-End OCFG_BID_OPERATIONS.
+(* TODO move to wherever lemmas about convert_typ get hosted  *)
 
+(* Lemma blk_id_map_convert_typ : forall env bs, *)
+(*     map blk_id (convert_typ env bs) = map blk_id bs. *)
+(* Proof. *)
+(*   induction bs as [| b bs IH]; cbn; auto. *)
+(*   f_equal; auto. *)
+(* Qed. *)
+
+(* Lemma wf_ocfg_bid_convert_typ : *)
+(*   forall env (bs : ocfg typ), *)
+(*     wf_ocfg_bid bs -> *)
+(*     wf_ocfg_bid (convert_typ env bs). *)
+(* Proof. *)
+(*   induction bs as [| b bs IH]; intros NOREP. *)
+(*   - cbn; auto. *)
+(*   - cbn. *)
+(*     apply list_norepet_cons.  *)
+(*     + cbn. *)
+(*       apply wf_ocfg_bid_cons_not_in in NOREP. *)
+(*       rewrite blk_id_map_convert_typ; auto. *)
+(*     + eapply IH, wf_ocfg_bid_cons; eauto.  *)
+(* Qed. *)
 
